@prefix :        <http://vocab.dhlab.epfl.ch/garzoni#> .
@prefix owl:     <http://www.w3.org/2002/07/owl#> .
@prefix rdf:     <http://www.w3.org/1999/02/22-rdf-syntax-ns#> .
@prefix xsd:     <http://www.w3.org/2001/XMLSchema#> .
@prefix skos:    <http://www.w3.org/2004/02/skos/core#> .
@prefix rdfs:    <http://www.w3.org/2000/01/rdf-schema#> .
@prefix grz:     <http://vocab.dhlab.epfl.ch/garzoni#> .

grz:relatedContract
      a       owl:ObjectProperty .

grz:Condition
      a       owl:Class ;
      rdfs:comment "Any condition or terms stated in a apprenticeship contract."^^xsd:anyURI ;
      rdfs:label "Condition"@fr , "Condition"@en .

<http://vocab.dhlab.epfl.ch/garzoni#Other_(currency)>
      a       owl:NamedIndividual , grz:CurrencyType ;
      rdfs:label "'Other_(currency)'"@en .

grz:OtherSalary
      a       grz:FinancialConditionType , owl:NamedIndividual ;
      rdfs:label "OtherSalary"@en .

grz:details
      a       owl:DatatypeProperty ;
      rdfs:comment "This property allows to state additionnal details about whatever."@en ;
      rdfs:label "details"@en ;
      rdfs:range xsd:string ;
      rdfs:subPropertyOf owl:topDataProperty .

grz:City
      a       grz:PlaceType , owl:NamedIndividual ;
      rdfs:label "City"@en .

grz:PlaceType
      a       owl:Class ;
      rdfs:comment "The type of place."@en ;
      rdfs:label "PlaceType"@en ;
      rdfs:subClassOf <http://semanticweb.cs.vu.nl/2009/11/sem/Type> ;
      owl:equivalentClass
              [ a       owl:Class ;
                owl:oneOf (grz:City grz:Country grz:Region grz:RuralArea)
              ] .

grz:hasWorkshop
      a       owl:ObjectProperty ;
      rdfs:comment "The relation between a PersonMention or PersonEntity and a Workshop."@en ;
      owl:inverseOf grz:isWorkshopOf .

grz:AppellationComponent
      a       owl:Class ;
      rdfs:comment "This class defines elements which compose the appellation, or name, of an entity."@en ;
      rdfs:label "AppellationComponent"@en , "Composant d'appellation"@fr .

grz:hasProfession
      a       owl:ObjectProperty ;
      rdfs:comment "This property allows to state the profession of a PersonMention or PersonEntity."@en .

grz:hasGeographicalOrigin
      a       owl:ObjectProperty ;
      rdfs:comment "This property allows to specific the geographical origins of a PersonMention or PersonEntity."@en .

<http://vocab.dhlab.epfl.ch/data-core#Source>
      a       owl:Class ;
      rdfs:isDefinedBy <http://vocab.dhlab.epfl.ch/data-core#> ;
      rdfs:label "Source"@en .

grz:RuralArea
      a       grz:PlaceType , owl:NamedIndividual ;
      rdfs:label "RuralArea"@en .

grz:id
      a       owl:DatatypeProperty ;
      rdfs:label "id"@en .

grz:hasMargin
      a       owl:DatatypeProperty ;
      rdfs:comment "This property allows to state whether a contract, in the register where it is written, has a complementary note in the margin or not."@en ;
      rdfs:domain grz:Contract ;
      rdfs:label "hasMargin"@en ;
      rdfs:range xsd:boolean .

grz:Apprenticeship
      a       grz:EventType , owl:NamedIndividual ;
      rdfs:comment "An event which corresponds to the execution of an apprenticeship."@en ;
      rdfs:label "Apprenticeship"@en , "Apprentissage"@fr .

<http://vocab.dhlab.epfl.ch/data-core#Mention>
      a       owl:Class ;
      rdfs:isDefinedBy "http://vocab.dhlab.epfl.ch/data-core#Mention"^^xsd:anyURI ;
      rdfs:label "Mention"@en .

grz:Country
      a       grz:PlaceType , owl:NamedIndividual ;
      rdfs:label "Country"@en .

grz:PersonalCare
      a       grz:HostingConditionType , owl:NamedIndividual ;
      rdfs:label "PersonalCare"@en .

grz:hasResidence
      a       owl:ObjectProperty ;
      rdfs:comment "This property allows to specify the residence of a PersonMention or PersonEntity."@en .

grz:SemestralPeriod
      a       grz:PeriodizationType , owl:NamedIndividual ;
      rdfs:label "SemestralPeriod"@en .

grz:Collectivename
      a       owl:Class ;
      rdfs:comment "In Garzoni context, this class covers expressions used to refer to collective entities. Typical examples include: \"et fratelli\" (and brothers), \"e fioli\", \"et sua consorte\" ."@en ;
      rdfs:label "Collectivename"@en , "Nom collectif"@fr ;
      rdfs:subClassOf grz:AppellationComponent .

grz:SingleSalary
      a       grz:FinancialConditionType , owl:NamedIndividual ;
      rdfs:comment "In a professional contractual setting, a fixed regular payment due by an employer to an employee."@en ;
      rdfs:label "SingleSalary"@en .

grz:oid
      a       owl:DatatypeProperty ;
      rdfs:comment "This property allows to state the object id of the mongo database (only valid for data coming from MediaWiki, should disappear.)"@en ;
      rdfs:domain grz:Contract ;
      rdfs:label "oid"@en .

grz:period
      a       owl:DatatypeProperty ;
      rdfs:comment "The period during which something happens."@en ;
      rdfs:domain grz:HostingCondition , grz:FinancialCondition ;
      rdfs:label "period"@en ;
      rdfs:range xsd:string .

<http://vocab.dhlab.epfl.ch/garzoni>
      a       owl:Ontology ;
      rdfs:comment "An ontology which models the information contained in the archival series \"Accordi dei Garzoni\" of the Venetian State Archives, relative to early modern venetian apprenticeship domain."@en ;
      rdfs:label "Garzoni Ontology"@en ;
      owl:versionIRI <http://vocab.dhlab.epfl.ch/garzoni> ;
      owl:versionInfo "1.0"^^xsd:float .

<http://vocab.dhlab.epfl.ch/data-core#Entity>
      a       owl:Class ;
      rdfs:isDefinedBy <http://vocab.dhlab.epfl.ch/data-core#Entity> ;
      rdfs:label "Entity"@en .

grz:MasterPayer
      a       owl:NamedIndividual , grz:PayerType ;
      rdfs:label "MasterPayer"@en .

grz:Patronymic1
      a       owl:Class ;
      rdfs:comment """Part of the name of a person which refers to one of his/her immediate relative. In (former) Italian family names, the patronymic is preceded by the word \"di\" or \"quondam\", e.g. \"Federico Di Garla\".
\"Di\" stands for \"figlio/figlia di\" or \"marito/moglie di\" meaning the son/daughter or husband/wife of a living person. \"Quondam\" means the same but for a person who ceased to live."""@en ;
      rdfs:label "Patronym1"@en , "Patronyme1"@fr ;
      rdfs:subClassOf grz:AppellationComponent .

grz:onMultiplePages
      a       owl:DatatypeProperty ;
      rdfs:comment "This property allows to state whether a contract spans over 2 pages or not."@en ;
      rdfs:domain grz:Contract ;
      rdfs:label "onMultiplePages"@en ;
      rdfs:range xsd:boolean .

grz:PayerType
      a       owl:Class ;
      rdfs:comment "The type of payer; in garzoni context, this is used to specify who is paying the apprenticeship: the apperntice to the master (emphasize on training), or the master to the apprentice (emphasize on employing)."@en ;
      rdfs:label "PayerType"@en ;
      rdfs:subClassOf <http://semanticweb.cs.vu.nl/2009/11/sem/Type> ;
      owl:equivalentClass
              [ a       owl:Class ;
                owl:oneOf (grz:ApprenticePayer grz:MasterPayer grz:OtherPayer)
              ] .

grz:Workshop
      a       owl:Class ;
      rdfs:comment "The place where objects are crafted or manufactured. In garzoni context, the place were the training of the apprentice was taking place."@en ;
      rdfs:label """Workshop
"""^^xsd:string , "Atelier"@fr ;
      rdfs:subClassOf <http://vocab.dhlab.epfl.ch/data-core#Entity> .

grz:hasNextPart
      a       owl:ObjectProperty ;
      rdfs:comment "This property allows to relate the different parts of a contract spanning over 2 pages."@en .

grz:ProgressiveSalary
      a       grz:FinancialConditionType , owl:NamedIndividual ;
      rdfs:label "ProgressiveSalary"@en .

grz:EventType
      a       owl:Class ;
      rdfs:comment "The type of event."@en ;
      rdfs:isDefinedBy <http://semanticweb.cs.vu.nl/2009/11/sem/EventType> ;
      rdfs:label "EventType"@en ;
      rdfs:subClassOf <http://semanticweb.cs.vu.nl/2009/11/sem/Type> ;
      owl:equivalentClass
              [ a       owl:Class ;
                owl:oneOf (grz:Apprenticeship grz:BreachOfContract grz:Enrolment grz:Flee)
              ] .

grz:conditionType
      a       owl:FunctionalProperty , owl:ObjectProperty ;
      rdfs:comment "This property allows to state the specific type of a  financial or hosting condition."@en ;
      rdfs:domain grz:Condition .

grz:professionCategory
      a       owl:DatatypeProperty ;
      rdfs:domain grz:ProfessionMention ;
      rdfs:label "professionCategory"@en ;
      rdfs:range xsd:string .

grz:WeeklyPeriod
      a       grz:PeriodizationType , owl:NamedIndividual ;
      rdfs:label "WeeklyPeriod"@en .

grz:hasCondition
      a       owl:ObjectProperty ;
      rdfs:domain grz:Contract ;
      rdfs:label "This property allows to assign a condition to a garzoni contract."@en ;
      rdfs:range grz:Condition ;
      owl:inverseOf grz:isConditionOf .

grz:ageText
      a       owl:DatatypeProperty ;
      rdfs:comment "To be deleted, only in MediaWiki"@en ;
      rdfs:label "ageText"@en ;
      rdfs:range xsd:string .

grz:Enrolment
      a       grz:EventType , owl:NamedIndividual ;
      rdfs:comment "An event which corresponds to the enrolment of an apprenticship. In the Garzoni project, it corresponds to the registration of the contract at the institution of the Giustizia Vecchia."@en ;
      rdfs:label "Inscription"@fr , "Enrolment"@en .

grz:Master
      a       owl:NamedIndividual , grz:RoleType ;
      rdfs:comment "A role or function which a person has while being a master duting an apprenticship."@en ;
      rdfs:label "Master"@en .

grz:ApprenticePayer
      a       owl:NamedIndividual , grz:PayerType ;
      rdfs:label "ApprenticePayer"@en .

grz:hasName
      a       owl:ObjectProperty ;
      rdfs:comment "This property is used to attribute a PersonAppellation to a PersonMention or a PersonEntity."^^xsd:anyURI ;
      rdfs:label "hasName"@en ;
      rdfs:range grz:PersonAppellation ;
      rdfs:seeAlso "http://www.cidoc-crm.org/html/5.0.4/cidoc-crm.html#P1"^^xsd:anyURI .

grz:ApplicationRule
      a       owl:Class ;
      rdfs:comment "The definition of the conditions under which a rule applies."@en ;
      rdfs:label "ApplicationRule"@en ;
      rdfs:subClassOf <http://semanticweb.cs.vu.nl/2009/11/sem/Type> ;
      owl:equivalentClass
              [ a       owl:Class ;
                owl:oneOf (grz:SanoApplication grz:SanoInfermoApplication)
              ] .

grz:Patronymic2
      a       owl:Class ;
      rdfs:comment """Part of the name of a person which refers to one of his/her relative. In (former) Italian family names, the patronymic is preceded by the word \"di\" or \"quondam\", e.g. \"Federico Di Garla\".
\"Di\" stands for \"figlio/figlia di\" or \"marito/moglie di\" meaning the son/daughter or husband/wife of a living person. \"Quondam\" means the same but for a person who ceased to live."""^^xsd:anyURI ;
      rdfs:label "Patronymic2"@fr ;
      rdfs:subClassOf grz:AppellationComponent .

grz:Surname
      a       owl:Class ;
      rdfs:comment "The surname or family name of a person entity."@en ;
      rdfs:label "Nom de famille"@fr , "Surname"@en ;
      rdfs:seeAlso "http://xmlns.com/foaf/0.1/familyName"^^xsd:anyURI ;
      rdfs:subClassOf grz:AppellationComponent .

grz:site
      a       owl:DatatypeProperty ;
      rdfs:comment "This property allows to state a complementary information relative to the location of a worshop."@en ;
      rdfs:label "site"@en .

grz:SanoApplication
      a       owl:NamedIndividual , grz:ApplicationRule ;
      rdfs:label "SanoApplication"@en .

grz:OtherPayer
      a       owl:NamedIndividual , grz:PayerType ;
      rdfs:label "OtherPayer"@en .

grz:Charge
      a       owl:Class ;
      rdfs:comment "A public responsibility hold by a person, usually different from his/her profession."@en ;
      rdfs:label """Charge
"""^^xsd:string ;
      rdfs:subClassOf <http://vocab.dhlab.epfl.ch/data-core#Entity> .

grz:currencyUnit
      a       owl:DatatypeProperty ;
      rdfs:comment "To be deleted when harmonization with Wiki fully done."@en ;
      rdfs:label "currencyUnit"@en .

grz:worksFor
      a       owl:DatatypeProperty ;
      rdfs:comment "This allow to state an additional information related to a ProfessionMention."@en ;
      rdfs:label "worksFor"@en ;
      rdfs:range xsd:string .

grz:applicationRule
      a       owl:DatatypeProperty ;
      rdfs:comment "This property allows to state the condition under which a rule is applied."@en ;
      rdfs:domain grz:HostingCondition ;
      rdfs:label "applicationRule"@en ;
      rdfs:range
              [ a       rdfs:Datatype ;
                owl:oneOf
                        [ a       rdf:List ;
                          rdf:first "none" ;
                          rdf:rest
                                  [ a       rdf:List ;
                                    rdf:first "sano" ;
                                    rdf:rest
                                            [ a       rdf:List ;
                                              rdf:first "sano et infermo" ;
                                              rdf:rest ()
                                            ]
                                  ]
                        ]
              ] .

grz:totalAmount
      a       owl:DatatypeProperty ;
      rdfs:domain grz:FinancialCondition ;
      rdfs:label "totalAmount"@en ;
      rdfs:range xsd:integer .

grz:FinancialConditionType
      a       owl:Class ;
      rdfs:comment "The type of financial condition."@en ;
      rdfs:label "FinancialConditionType."@en ;
      rdfs:subClassOf <http://semanticweb.cs.vu.nl/2009/11/sem/Type> ;
      owl:equivalentClass
              [ a       owl:Class ;
                owl:oneOf (grz:Pledge grz:SingleSalary)
              ] .

grz:Ducati
      a       owl:NamedIndividual , grz:CurrencyType ;
      rdfs:label "Ducati"@en .

grz:MonthlyPeriod
      a       grz:PeriodizationType , owl:NamedIndividual ;
      rdfs:label "MonthlyPeriod"@en .

grz:DailyPeriod
      a       grz:PeriodizationType , owl:NamedIndividual ;
      rdfs:label "DailyPeriod"@en .

grz:Forename
      a       owl:Class ;
      rdfs:comment "The firstname of a person."@en ;
      rdfs:label "Firstname"@en , "Pr√©nom"@fr ;
      rdfs:seeAlso "http://xmlns.com/foaf/0.1/givenName"^^xsd:anyURI ;
      rdfs:subClassOf grz:AppellationComponent .

grz:Apprentice
      a       owl:NamedIndividual , grz:RoleType ;
      rdfs:comment "A role or function which a person has when being enrolled as apprentice during an apprenticeship."@en ;
      rdfs:label "Apprentice"@en .

grz:quondam1
      a       owl:DatatypeProperty , owl:FunctionalProperty ;
      rdfs:comment "This property allows to state the status of the first quondam information in an Appellation. If 'di', then false, otherwise true."@en ;
      rdfs:domain grz:PersonAppellation ;
      rdfs:label "quondam1"@en ;
      rdfs:range xsd:boolean .

grz:clothingType
      a       owl:DatatypeProperty ;
      rdfs:comment "An indication on the type of clothes which is being paid to an apprentice."@en ;
      rdfs:domain grz:HostingCondition ;
      rdfs:label "clothingType"@en ;
      rdfs:range xsd:string .

grz:Soldi
      a       owl:NamedIndividual , grz:CurrencyType ;
      rdfs:label "Soldi"@en .

grz:isWorkshopOf
      a       owl:ObjectProperty ;
      rdfs:domain grz:WorkshopMention ;
      rdfs:label "isWorkshopOf"@en .

grz:hasCharge
      a       owl:ObjectProperty ;
      rdfs:label "This property allows to assign a charge to a PersonMention or a PersonEntity."@en .

grz:Profession
      a       owl:Class ;
      rdfs:comment "Activity in which someone is skilled and which is carries out in order to make a living. Occupation."@en ;
      rdfs:label "Profession"@fr , "Profession"@en ;
      rdfs:subClassOf <http://vocab.dhlab.epfl.ch/data-core#Entity> .

grz:HostingCondition
      a       owl:Class ;
      rdfs:comment "The contract's terms relative to hosting, i.e. some benefit in kind."@en ;
      rdfs:label "HostingCondition"@en ;
      rdfs:subClassOf grz:Condition ;
      owl:equivalentClass
              [ a       owl:Restriction ;
                owl:allValuesFrom grz:HostingConditionType ;
                owl:onProperty grz:conditionType
              ] .

grz:hasRole
      a       owl:ObjectProperty ;
      rdfs:isDefinedBy "This property specifies the role of a PersonMention or PersonEntity."@en .

grz:mediaWikiReference
      a       owl:DatatypeProperty ;
      rdfs:comment "This property allows to link a contract to its corresponding object contract in the former MediaWiki database."@en ;
      rdfs:label "mediaWikiReference"@en .

grz:paidInGoods
      a       owl:DatatypeProperty ;
      rdfs:domain grz:HostingCondition , grz:FinancialCondition ;
      rdfs:label "paidInGoods"@en ;
      rdfs:range xsd:boolean .

grz:quondam2
      a       owl:DatatypeProperty , owl:FunctionalProperty ;
      rdfs:comment "This property allows to state the status of the second quondam information in an Appellation."@en ;
      rdfs:domain grz:PersonAppellation ;
      rdfs:label "quondam2"@en ;
      rdfs:range xsd:boolean .

grz:denunciationDate
      a       owl:DatatypeProperty ;
      rdfs:comment "This property allows to state at which date a flee has been denounced."@en ;
      rdfs:label "denunciationDate"@en .

grz:Other
      a       owl:NamedIndividual , grz:RoleType ;
      rdfs:comment "An undetermined role or function taht a person has."@en ;
      rdfs:label "Other"@en .

grz:SanoInfermoApplication
      a       owl:NamedIndividual , grz:ApplicationRule ;
      rdfs:label "SanoInfermoApplication"@en .

grz:GenericExpenses
      a       grz:HostingConditionType , owl:NamedIndividual ;
      rdfs:label "GenericExpenses"@en .

grz:identifiedPerson
      a       owl:DatatypeProperty ;
      rdfs:comment "To be deleted, only in MediaWiki."@en ;
      rdfs:label "identifiedPerson"@en ;
      rdfs:range xsd:string .

<http://semanticweb.cs.vu.nl/2009/11/sem/Type>
      a       owl:Class ;
      rdfs:isDefinedBy <http://semanticweb.cs.vu.nl/2009/11/sem/Type> ;
      rdfs:label "Type"@en .

grz:PeriodizationType
      a       owl:Class ;
      rdfs:comment "The type of periodization; in garzoni context, this is used to specify at which intervals the salary is paid."@en ;
      rdfs:label "PeriodizationType"@en ;
      rdfs:subClassOf <http://semanticweb.cs.vu.nl/2009/11/sem/Type> ;
      owl:equivalentClass
              [ a       owl:Class ;
                owl:oneOf (grz:AnnualPeriod grz:DailyPeriod grz:MonthlyPeriod grz:SemestralPeriod grz:WeeklyPeriod grz:WholePeriod)
              ] .

grz:WorkshopMention
      a       owl:Class ;
      rdfs:comment "The mention of a workshop."@en ;
      rdfs:label "WorkshopMention"@en ;
      rdfs:subClassOf <http://vocab.dhlab.epfl.ch/data-core#Mention> .

grz:Pledge
      a       grz:FinancialConditionType , owl:NamedIndividual ;
      rdfs:label "Pledge"@en .

grz:PersonAppellation
      a       owl:Class ;
      rdfs:comment "The name of a person entity."^^xsd:string ;
      rdfs:label "PersonAppellation"@en ;
      rdfs:seeAlso "http://www.cidoc-crm.org/html/5.0.4/cidoc-crm.html#E41"^^xsd:anyURI .

grz:ProfessionMention
      a       owl:Class ;
      rdfs:comment "The mention of the profession of a person."@en ;
      rdfs:label "ProfessionMention"@en ;
      rdfs:subClassOf <http://vocab.dhlab.epfl.ch/data-core#Mention> .

grz:Lire
      a       owl:NamedIndividual , grz:CurrencyType ;
      rdfs:label "Lire"@en .

grz:moneyInformation
      a       owl:DatatypeProperty ;
      rdfs:comment "Additional information about money, if necessary."@en ;
      rdfs:domain grz:FinancialCondition ;
      rdfs:label "moneyInformation"@en ;
      rdfs:range xsd:string .

grz:Flee
      a       grz:EventType , owl:NamedIndividual ;
      rdfs:comment "An event which corresponds to the flee of an apprentice during its apprenticeship."@en ;
      rdfs:label "Flee"@en , "Fugue"@fr .

grz:Accommodation
      a       grz:HostingConditionType , owl:NamedIndividual ;
      rdfs:label "Accommodation"@en .

grz:BreachOfContract
      a       grz:EventType , owl:NamedIndividual ;
      rdfs:comment "An event which corresponds to the breaking of a contract."@en ;
      rdfs:label "Rupture de contrat"@fr , "BreachofContract"@en .

grz:paidBy
      a       owl:DatatypeProperty ;
      rdfs:domain grz:HostingCondition , grz:FinancialCondition ;
      rdfs:label "paidBy"@en ;
      rdfs:range
              [ a       rdfs:Datatype ;
                owl:oneOf
                        [ a       rdf:List ;
                          rdf:first "apprentice" ;
                          rdf:rest
                                  [ a       rdf:List ;
                                    rdf:first "master" ;
                                    rdf:rest
                                            [ a       rdf:List ;
                                              rdf:first "nobody" ;
                                              rdf:rest
                                                      [ a       rdf:List ;
                                                        rdf:first "other" ;
                                                        rdf:rest ()
                                                      ]
                                            ]
                                  ]
                        ]
              ] .

grz:RoleType
      a       owl:Class ;
      rdfs:comment "The type of role."@en ;
      rdfs:isDefinedBy <http://semanticweb.cs.vu.nl/2009/11/sem/RoleType> ;
      rdfs:label "RoleType"@en ;
      rdfs:subClassOf <http://semanticweb.cs.vu.nl/2009/11/sem/Type> ;
      owl:equivalentClass
              [ a       owl:Class ;
                owl:oneOf (grz:Apprentice grz:Guarantor grz:Master grz:Other)
              ] .

grz:Clothing
      a       grz:HostingConditionType , owl:NamedIndividual ;
      rdfs:label "Clothing"@en .

grz:Contract
      a       owl:Class ;
      rdfs:comment "A legal agreement between parties that set up the conditions of an employment. In the Garzoni project, this corresponds to an apprenticeship contract between a master and an apprentice with, often, the caution of a guarantor."@en ;
      rdfs:label "Contract"^^xsd:string , "Contrat"@fr ;
      rdfs:subClassOf <http://vocab.dhlab.epfl.ch/data-core#Source> .

grz:isNextPartOf
      a       owl:ObjectProperty ;
      rdfs:domain grz:Contract ;
      rdfs:label "isNextPartOf"@en ;
      rdfs:range grz:Contract .

grz:ChargeMention
      a       owl:Class ;
      rdfs:comment "The mention of a Charge."@en ;
      rdfs:label "ChargeMention"@en ;
      rdfs:subClassOf <http://vocab.dhlab.epfl.ch/data-core#Mention> .

grz:periodization
      a       owl:DatatypeProperty ;
      rdfs:comment "The regular time period at which something happens."@en ;
      rdfs:domain grz:HostingCondition , grz:FinancialCondition ;
      rdfs:label "Periodization"@en ;
      rdfs:range
              [ a       rdfs:Datatype ;
                owl:oneOf
                        [ a       rdf:List ;
                          rdf:first "annual" ;
                          rdf:rest
                                  [ a       rdf:List ;
                                    rdf:first "daily" ;
                                    rdf:rest
                                            [ a       rdf:List ;
                                              rdf:first "monthly" ;
                                              rdf:rest
                                                      [ a       rdf:List ;
                                                        rdf:first "none" ;
                                                        rdf:rest
                                                                [ a       rdf:List ;
                                                                  rdf:first "semestral" ;
                                                                  rdf:rest
                                                                          [ a       rdf:List ;
                                                                            rdf:first "weekly" ;
                                                                            rdf:rest
                                                                                    [ a       rdf:List ;
                                                                                      rdf:first "whole period" ;
                                                                                      rdf:rest ()
                                                                                    ]
                                                                          ]
                                                                ]
                                                      ]
                                            ]
                                  ]
                        ]
              ] .

grz:placeType
      a       owl:ObjectProperty ;
      rdfs:label "placeType"@en .

grz:HostingConditionType
      a       owl:Class ;
      rdfs:comment "The type of hosting condition."@en ;
      rdfs:label "HostingConditionType"@en ;
      rdfs:subClassOf <http://semanticweb.cs.vu.nl/2009/11/sem/Type> ;
      owl:equivalentClass
              [ a       owl:Class ;
                owl:oneOf (grz:Accommodation grz:Clothing grz:GenericExpenses grz:PersonalCare)
              ] .

grz:Region
      a       grz:PlaceType , owl:NamedIndividual ;
      rdfs:label "Region"@en .

grz:Guarantor
      a       owl:NamedIndividual , grz:RoleType ;
      rdfs:comment "A role or function that a person has while being a guarantor in the context of an apprenticeship."@en ;
      rdfs:label "Guarantor"@en .

grz:insigna
      a       owl:DatatypeProperty ;
      rdfs:comment "This property allows to state the emblem or 'name' of a workshop."@en ;
      rdfs:domain grz:WorkshopMention ;
      rdfs:label "insigna"@en ;
      rdfs:range xsd:string .

grz:FinancialCondition
      a       owl:Class ;
      rdfs:comment "The financial terms of a contract."@en ;
      rdfs:label "FinancialCondition"@en ;
      rdfs:subClassOf grz:Condition ;
      owl:equivalentClass
              [ a       owl:Restriction ;
                owl:allValuesFrom grz:FinancialConditionType ;
                owl:onProperty grz:conditionType
              ] .

grz:partialAmount
      a       owl:DatatypeProperty ;
      rdfs:comment "The partial amount of a progressive salary."@en ;
      rdfs:domain grz:FinancialCondition ;
      rdfs:label "partialAmount"@en ;
      rdfs:range xsd:integer .

grz:isConditionOf
      a       owl:FunctionalProperty , owl:ObjectProperty ;
      rdfs:domain grz:Condition ;
      rdfs:label "isConditionOf"@en ;
      rdfs:range grz:Contract .

grz:WholePeriod
      a       grz:PeriodizationType , owl:NamedIndividual ;
      rdfs:label "WholePeriod"@en .

grz:hasLocation
      a       owl:ObjectProperty ;
      rdfs:comment "This property allows to specify the location of an entity" ;
      rdfs:domain grz:WorkshopMention ;
      rdfs:isDefinedBy <http://www.ontologydesignpatterns.org/cp/owl/place.owl> ;
      rdfs:label "hasLocation"@en ;
      rdfs:subPropertyOf owl:topObjectProperty .

grz:CurrencyType
      a       owl:Class ;
      rdfs:comment "The type of currency."@en ;
      rdfs:label "CurrencyType"@en ;
      rdfs:subClassOf <http://semanticweb.cs.vu.nl/2009/11/sem/Type> ;
      owl:equivalentClass
              [ a       owl:Class ;
                owl:oneOf (grz:Ducati grz:Lire grz:Soldi <http://vocab.dhlab.epfl.ch/garzoni#Other_(currency)>)
              ] .

grz:AnnualPeriod
      a       grz:PeriodizationType , owl:NamedIndividual ;
      rdfs:label "AnnualPeriod"@en .
